code/api/Hacl.SecretBox.ZeroPad.fst
@@ -1,5 +1,6 @@
 module Hacl.SecretBox.ZeroPad
 
+open FStar.HyperStack
 open FStar.Buffer
 open FStar.ST
 open Hacl.Constants
@@ -15,6 +16,9 @@ module U64 = FStar.UInt64
 module H8  = Hacl.UInt8
 module H32 = Hacl.UInt32
 module H64 = Hacl.UInt64
+
+
+#reset-options "--initial_fuel 0 --max_fuel 0 --z3rlimit 50"
 
 private val set_zero_bytes:
   b:uint8_p{length b >= 32} ->
@@ -32,66 +36,91 @@ let set_zero_bytes b =
   b.(24ul) <- zero; b.(25ul) <- zero; b.(26ul) <- zero; b.(27ul) <- zero;
   b.(28ul) <- zero; b.(29ul) <- zero; b.(30ul) <- zero; b.(31ul) <- zero
 
+#reset-options "--initial_fuel 0 --max_fuel 0 --z3rlimit 100"
+
+private val lemma_crypto_secretbox_detached:
+  h0:mem -> h2:mem -> h3:mem -> h4:mem -> h5:mem -> h6:mem ->
+  sk:uint8_p -> mac:uint8_p -> c:uint8_p ->
+  Lemma (requires (~(contains h0 sk) /\ live h0 mac /\ live h0 c /\ modifies_0 h0 h2
+    /\ modifies_1 c h2 h3 /\ modifies_1 mac h3 h4 /\ modifies_1 c h4 h5 /\ modifies_1 sk h5 h6
+    /\ live h2 sk /\ live h2 mac /\ live h2 c
+    /\ live h3 sk /\ live h3 mac /\ live h3 c
+    /\ live h4 sk /\ live h4 mac /\ live h4 c
+    /\ live h5 sk /\ live h5 mac /\ live h5 c
+    /\ live h5 sk /\ live h6 mac /\ live h6 c
+    ))
+        (ensures (modifies_3_2 c mac h0 h6))
+private let lemma_crypto_secretbox_detached h0 h2 h3 h4 h5 h6 sk mac c =
+  lemma_reveal_modifies_0 h0 h2;
+  lemma_reveal_modifies_1 c h2 h3;
+  lemma_reveal_modifies_1 mac h3 h4;
+  lemma_reveal_modifies_1 c h4 h5;
+  lemma_reveal_modifies_1 sk h5 h6;
+  lemma_intro_modifies_3_2 c mac h0 h6
+
+
 #reset-options "--initial_fuel 0 --max_fuel 0 --z3rlimit 50"
+
 (* We assume that the first 32 bytes of c and m are 0s and will remain 0s *)
 val crypto_secretbox_detached:
   c:uint8_p ->
   mac:uint8_p{length mac = crypto_secretbox_MACBYTES /\ disjoint mac c} ->
   m:uint8_p ->
-  mlen:u64{let len = U64.v mlen in len = length m /\ len = length c}  ->
+  mlen:u64{let len = U64.v mlen in len + 32 = length m /\ len + 32 = length c}  ->
   n:uint8_p{length n = crypto_secretbox_NONCEBYTES} ->
   k:uint8_p{length k = crypto_secretbox_KEYBYTES} ->
   Stack u32
     (requires (fun h -> live h c /\ live h mac /\ live h m /\ live h n /\ live h k))
     (ensures  (fun h0 z h1 -> modifies_2 c mac h0 h1 /\ live h1 c /\ live h1 mac))
+#reset-options "--initial_fuel 0 --max_fuel 0 --z3rlimit 100"
 let crypto_secretbox_detached c mac m mlen n k =
+  let mlen_ = Int.Cast.uint64_to_uint32 mlen in
+  Math.Lemmas.modulo_lemma (U64.v mlen) (pow2 32);
   let hinit = ST.get() in
   push_frame();
   let h0 = ST.get() in
   let subkey = create (uint8_to_sint8 0uy) 32ul in
-  let h0' = ST.get() in
+  let h1 = ST.get() in
   Hacl.Symmetric.HSalsa20.crypto_core_hsalsa20 subkey (sub n 0ul 16ul) k;
+  let h2 = ST.get() in
   Salsa20.crypto_stream_salsa20_xor c
                                     m
                                     U64.(mlen +^ 32uL)
                                     (sub n 16ul 8ul)
                                     subkey;
-  let mlen_ = Int.Cast.uint64_to_uint32 mlen in
+  let h3 = ST.get() in
   Poly1305_64.crypto_onetimeauth mac (sub c 32ul mlen_) mlen (sub c 0ul 32ul);
+  let h4 = ST.get() in
   set_zero_bytes(c);
+  let h5 = ST.get() in
   set_zero_bytes(subkey);
+  let h6 = ST.get() in
+  lemma_crypto_secretbox_detached h0 h2 h3 h4 h5 h6 subkey mac c;
   pop_frame();
   0ul
 
 
 #reset-options "--initial_fuel 0 --max_fuel 0 --z3rlimit 200"
 
-(* We assume that the first 32 bytes of m and c are 0 *)
-val crypto_secretbox_open_detached:
+private let lemma_crypto_secretbox_open_detached_decrypt (h:mem) (m:uint8_p) (subkey:uint8_p) :
+  Lemma (modifies_2 m subkey h h)
+  = lemma_intro_modifies_2 m subkey h h
+
+
+#reset-options "--initial_fuel 0 --max_fuel 0 --z3rlimit 200"
+
+private val crypto_secretbox_open_detached_decrypt:
   m:uint8_p ->
-  c:uint8_p ->
-  mac:uint8_p{length mac = crypto_secretbox_MACBYTES /\ declassifiable mac} ->
-  clen:u64{let len = U64.v clen in len = length m /\ len = length c}  ->
+  c:uint8_p{disjoint c m} ->
+  clen:u64{let len = U64.v clen in len + 32 = length m /\ len + 32 = length c}  ->
   n:uint8_p{length n = crypto_secretbox_NONCEBYTES} ->
-  k:uint8_p{length k = crypto_secretbox_KEYBYTES} ->
+  subkey:uint8_p{length subkey = 32 /\ disjoint m subkey} ->
+  verify:U8.t ->
   Stack u32
-    (requires (fun h -> live h m /\ live h c /\ live h mac /\ live h n /\ live h k))
-    (ensures  (fun h0 z h1 -> modifies_1 m h0 h1 /\ live h1 m))
-let crypto_secretbox_open_detached m c mac clen n k =
-  let hinit = ST.get() in
-  push_frame();
-  let h0 = ST.get() in
-  let subkey = create (uint8_to_sint8 0uy) 32ul in
-  let mackey = create (uint8_to_sint8 0uy) 64ul in
-  let cmac   = create (uint8_to_sint8 0uy) 16ul in
-  let h0' = ST.get() in
-  Hacl.Symmetric.HSalsa20.crypto_core_hsalsa20 subkey (sub n 0ul 16ul) k;
-  Salsa20.crypto_stream_salsa20 mackey 32uL (sub n 16ul 8ul) subkey;
-  let clen_ = Int.Cast.uint64_to_uint32 clen in
-  Poly1305_64.crypto_onetimeauth cmac (sub c 32ul clen_) clen mackey;
-  assume (Hacl.Policies.declassifiable cmac);
-  let verify = cmp_bytes mac cmac 16ul in
-  let z = 
+    (requires (fun h -> live h m /\ live h c /\ live h n /\ live h subkey))
+    (ensures (fun h0 _ h1 -> modifies_2 m subkey h0 h1 /\ live h1 m /\ live h1 subkey))
+let crypto_secretbox_open_detached_decrypt m c clen n subkey verify =
+    let h = ST.get() in
     if U8.(verify =^ 0uy) then (
       Salsa20.crypto_stream_salsa20_xor m
                                         c
@@ -101,23 +130,70 @@ let crypto_secretbox_open_detached m c mac clen n k =
       set_zero_bytes subkey;
       set_zero_bytes m;
       0ul)
-    else 0xfffffffful in
+    else (
+      lemma_crypto_secretbox_open_detached_decrypt h m subkey;
+      0xfffffffful
+    )
+
+
+(* We assume that the first 32 bytes of m and c are 0 *)
+val crypto_secretbox_open_detached:
+  m:uint8_p ->
+  c:uint8_p{disjoint m c} ->
+  mac:uint8_p{length mac = crypto_secretbox_MACBYTES /\ declassifiable mac} ->
+  clen:u64{let len = U64.v clen in len + 32 = length m /\ len + 32 = length c}  ->
+  n:uint8_p{length n = crypto_secretbox_NONCEBYTES} ->
+  k:uint8_p{length k = crypto_secretbox_KEYBYTES} ->
+  Stack u32
+    (requires (fun h -> live h m /\ live h c /\ live h mac /\ live h n /\ live h k))
+    (ensures  (fun h0 z h1 -> modifies_1 m h0 h1 /\ live h1 m))
+let crypto_secretbox_open_detached m c mac clen n k =
+  let hinit = ST.get() in
+  push_frame();
+  let h0 = ST.get() in
+  let tmp    = create (uint8_to_sint8 0uy) 112ul in
+  let subkey = Buffer.sub tmp 0ul 32ul in
+  let mackey = Buffer.sub tmp 32ul 64ul in
+  let cmac   = Buffer.sub tmp 96ul 16ul in
+  (* let subkey = create (uint8_to_sint8 0uy) 32ul in *)
+  (* let mackey = create (uint8_to_sint8 0uy) 64ul in *)
+  (* let cmac   = create (uint8_to_sint8 0uy) 16ul in *)
+  let h0' = ST.get() in
+  Hacl.Symmetric.HSalsa20.crypto_core_hsalsa20 subkey (sub n 0ul 16ul) k;
+  Salsa20.crypto_stream_salsa20 mackey 32uL (sub n 16ul 8ul) subkey;
+  let clen_ = Int.Cast.uint64_to_uint32 clen in
+  Poly1305_64.crypto_onetimeauth cmac (sub c 32ul clen_) clen (Buffer.sub mackey 0ul 32ul);
+  let h1 = ST.get() in
+  cut (modifies_0 h0 h1);
+  assume (Hacl.Policies.declassifiable cmac);
+  let verify = cmp_bytes mac cmac 16ul in
+  let z = crypto_secretbox_open_detached_decrypt m c clen n subkey verify in
+    (* if U8.(verify =^ 0uy) then ( *)
+    (*   Salsa20.crypto_stream_salsa20_xor m *)
+    (*                                     c *)
+    (*     				U64.(clen +^ 32uL) *)
+    (*     				(sub n 16ul 8ul) *)
+    (*                                 	subkey; *)
+    (*   set_zero_bytes subkey; *)
+    (*   set_zero_bytes m; *)
+    (*   0ul) *)
+    (* else 0xfffffffful in *)
   pop_frame();
   z
 
-#reset-options "--initial_fuel 0 --max_fuel 0 --z3rlimit 5"
+#reset-options "--initial_fuel 0 --max_fuel 0 --z3rlimit 20"
 
 val crypto_secretbox_easy:
   c:uint8_p ->
-  m:uint8_p ->
-  mlen:u64{let len = U64.v mlen in len <= length m /\ len + crypto_secretbox_MACBYTES <= length c}  ->
+  m:uint8_p{disjoint c m} ->
+  mlen:u64{let len = U64.v mlen in len + 32 = length m /\ len + 32 = length c}  ->
   n:uint8_p{length n = crypto_secretbox_NONCEBYTES} ->
   k:uint8_p{length k = crypto_secretbox_KEYBYTES} ->
   Stack u32
     (requires (fun h -> live h c /\ live h m /\ live h n /\ live h k))
     (ensures  (fun h0 z h1 -> modifies_1 c h0 h1 /\ live h1 c))
 let crypto_secretbox_easy c m mlen n k =
-  push_frame ();  
+  push_frame ();
   let mlen_ = FStar.Int.Cast.uint64_to_uint32 mlen in
   Math.Lemmas.modulo_lemma (U64.v mlen) (pow2 32);
   let cmac   = create (uint8_to_sint8 0uy) 16ul in
@@ -126,17 +202,18 @@ let crypto_secretbox_easy c m mlen n k =
   pop_frame();
   res
 
+
 val crypto_secretbox_open_easy:
   m:uint8_p ->
-  c:uint8_p ->
-  clen:u64{let len = U64.v clen in len = length m + crypto_secretbox_MACBYTES /\ len = length c}  ->
+  c:uint8_p{disjoint m c} ->
+  clen:u64{let len = U64.v clen in len + 32 = length m /\ len + 32 = length c}  ->
   n:uint8_p{length n = crypto_secretbox_NONCEBYTES} ->
   k:uint8_p{length k = crypto_secretbox_KEYBYTES} ->
   Stack u32
     (requires (fun h -> live h c /\ live h m /\ live h n /\ live h k))
     (ensures  (fun h0 z h1 -> modifies_1 m h0 h1 /\ live h1 m))
 let crypto_secretbox_open_easy m c clen n k =
-  let mac = sub c 16ul 16ul in
+  let mac = sub c 0ul 16ul in
   (* Declassification assumption (non constant-time operations may happen on the 'mac' buffer *)
   assume (declassifiable mac);
-  crypto_secretbox_open_detached m c mac U64.(clen -^ 16uL) n k
+  crypto_secretbox_open_detached m c mac U64.(clen) n k
